Add Increasing_In_powerset.
Of course this commit adds a number of other theorems as well, but
this is the main result. The way hypotheses of normalization are
satisfied is ugly, in particular because they need to be supplied
every time a theorem about normalization is used. But I do not
know a truly modular way to avoid this.

B1_utils.v
@@ -148,6 +148,13 @@ induction l; intros. easy. inv H.
   exists (a :: l1), l2; simpl; rewrite H; easy.
 Qed.
 
+Theorem Forall_incl {X} P (l l' : list X) :
+  (∀x, In x l -> In x l') -> Forall P l' -> Forall P l.
+Proof.
+intros; apply Forall_forall; intros.
+apply Forall_forall with (x:=x) in H0; auto.
+Qed.
+
 Notation lmax l := (fold_right max 0 l).
 
 Theorem lmax_in n l :
@@ -289,67 +296,6 @@ destruct (in_dec dec x l) as [H0|H0].
 1: exists (x :: l1), l2. 2: exists (a :: l1), l2. 3: exists [], l. all: easy.
 Qed.
 
-Section Powerset.
-
-Fixpoint powerset (u : list X) :=
-  match u with
-  | [] => [[]]
-  | a :: v => let p := powerset v in p ++ map (cons a) p
-  end.
-
-Fixpoint normalize (u l : list X) :=
-  match u with
-  | [] => []
-  | a :: v =>
-    let tl := normalize v (remove dec a l) in
-    if in_dec dec a l then a :: tl else tl
-  end.
-
-Theorem powerset_length u :
-  length (powerset u) = 2^length u.
-Proof.
-induction u; simpl. easy.
-now rewrite Nat.add_0_r, app_length, map_length, ?IHu.
-Qed.
-
-Theorem normalize_spec u l :
-  In (normalize u l) (powerset u).
-Proof.
-revert l; induction u; simpl; intros. now left.
-destruct (in_dec dec a l); apply in_app_iff; [right|left].
-apply in_map. all: apply IHu.
-Qed.
-
-Theorem normalize_sound u l x :
-  In x (normalize u l) -> In x l.
-Proof.
-revert l; induction u; simpl; intros. easy.
-destruct (in_dec dec a l); simpl. inv H; rename H0 into H.
-all: apply IHu, in_remove in H; easy.
-Qed.
-
-Theorem normalize_complete u l x :
-  In x u -> In x l -> In x (normalize u l).
-Proof.
-revert l; induction u; simpl; intros. easy.
-destruct (in_dec dec a l), (dec x a), H; simpl; subst; auto; try easy. right.
-all: apply IHu; [easy|]; apply in_in_remove; easy.
-Qed.
-
-Theorem normalize_normalize u l :
-  normalize u (normalize u l) = normalize u l.
-Proof.
-revert l; induction u; simpl; intros. easy.
-destruct (in_dec dec a l); simpl.
-destruct (dec a a); [|easy]. apply wd.
-2: destruct (in_dec _ _ _).
-2: apply normalize_sound, remove_In in i; easy.
-all: rewrite notin_remove; [apply IHu|].
-all: eapply contra; [apply normalize_sound|apply remove_In].
-Qed.
-
-End Powerset.
-
 Section Filtering.
 
 Variable P : X -> Prop.
@@ -460,8 +406,6 @@ End List_constructions_using_decidability.
 
 Arguments map2 {_ _ _}.
 Arguments strip {_}.
-Arguments powerset {_}.
-Arguments normalize {_}.
 Arguments pfilter {_}.
 Arguments intersect {_}.
 Arguments subtract {_}.
